Other spec

proofs/lean/extraction/Verif.lean
@@ -2,7 +2,9 @@ import extraction.Gcd
 open Std.Do
 open Std.Tactic
 
-@[spec]
+set_option mvcgen.warning false
+set_option linter.unusedVariables false
+
 theorem Rust_primitives.Hax.while_loop.spec {State: Type}
   (cond: State → Result Bool)
   (cond' : State → Bool)
@@ -51,6 +53,40 @@ theorem Rust_primitives.Hax.while_loop.spec {State: Type}
   ⦃ ⇓ state' => ⌜ inv' state' = true ∧ cond' state' = false ⌝ ⦄ := by sorry
 
 
+abbrev panic_free {α : Type} (f : Result α) := ⦃ ⌜ True ⌝ ⦄ f ⦃ ⇓ _ => ⌜ True ⌝ ⦄
+
+theorem Rust_primitives.Hax.while_loop.spec2 {State: Type}
+  (cond: State → Result Bool)
+  (inv: State → Result Bool)
+  (termination : State -> Result Int)
+  (init : State)
+  (body : State -> Result State)
+  (inv_init_true :
+    ⊢ₛ wp⟦ inv init ⟧ (⇓ r => ⌜ ↑r ⌝ ))
+  (inv_implies_cond_pf : ∀ state,
+    ⊢ₛ wp⟦ inv state ⟧ ( ⇓ r => ⌜ r → panic_free (cond state) ⌝ ))
+  (step : ∀ state,
+    ⊢ₛ wp⟦ inv state ⟧ post⟨
+      fun r => ⌜ r → ⊢ₛ wp⟦
+        do
+          if (← cond state) then
+            let state' ← (body state)
+            let m ← (termination state)
+            let m' ← (termination state')
+            pure ((← inv state') ∧ 0 ≤ m' ∧ m' < m)
+          else
+            pure true
+        ⟧ ( ⇓ r => ⌜ ↑r ⌝) ⌝ ,
+      fun _ => ⌜ True ⌝ -- if the invariant panics, nothing to do
+      ⟩) :
+  ⦃ ⌜ True ⌝ ⦄
+  Rust_primitives.Hax.while_loop cond inv termination init body
+  ⦃ ⇓ state' => ⌜
+    (⊢ₛ wp⟦inv state'⟧ (⇓ r => ⌜ r ⌝)) ∧
+    (⊢ₛ wp⟦cond state'⟧ ( ⇓ r => ⌜ ¬r ⌝))⌝ ⦄ := by sorry
+
+
+
 @[spec]
 theorem Hax.rem (a:u8) (b:u8) (hb :b ≠ 0) :
   ⦃ ⌜ True ⌝ ⦄
@@ -58,20 +94,16 @@ theorem Hax.rem (a:u8) (b:u8) (hb :b ≠ 0) :
   ⦃ ⇓ r => ⌜ r < b ⌝ ⦄
   := sorry
 
-
 theorem Gcd.euclid_u8.spec (a:u8) (b:u8) :
   ⦃ ⌜ True ⌝ ⦄
   (euclid_u8 a b)
   ⦃ ⇓ r => ⌜ True ⌝ ⦄
   := by
-  mvcgen (stepLimit := none) [euclid_u8]
-  · grind
-  · grind
-  · constructor
-    apply Int.zero_le_ofNat
-    exact Int.lt_of_toNat_lt (by assumption)
-  · grind
-  · grind
-  · constructor
-    apply Int.zero_le_ofNat
-    exact Int.lt_of_toNat_lt (by assumption)
+  mvcgen [euclid_u8, Rust_primitives.Hax.while_loop.spec2, panic_free]
+  <;> try mvcgen
+  <;> simp
+  <;> try grind
+  . apply UInt8.lt_iff_toNat_lt.mp
+    omega
+  . apply UInt8.lt_iff_toNat_lt.mp
+    omega
